Stabilize Hacl.Spec.Poly1305.Equiv by disabling non-lineari arithmetic

code/poly1305/Hacl.Spec.Poly1305.Equiv.fst
@@ -14,7 +14,7 @@ module S = Spec.Poly1305
 
 include Hacl.Spec.Poly1305.Vec
 
-#set-options "--z3rlimit 50 --max_fuel 0 --max_ifuel 0"
+#reset-options "--z3rlimit 50 --fuel 0 --ifuel 0 --z3cliopt smt.arith.nl=false"
 
 let block_v (w:lanes{w * size_block <= max_size_t}) = lbytes (w * size_block)
 
@@ -24,7 +24,8 @@ let block_v (w:lanes{w * size_block <= max_size_t}) = lbytes (w * size_block)
 ///
 
 val load_acc_lemma1: b:block_v 1 -> acc0:pfelem -> r:pfelem -> Lemma
-  (normalize_n r (load_acc #1 b acc0) ==
+  (Math.Lemmas.multiple_modulo_lemma 1 size_block;
+  normalize_n r (load_acc #1 b acc0) ==
    repeat_blocks_multi size_block b (S.poly1305_update1 r size_block) acc0)
 
 let load_acc_lemma1 b acc0 r =
@@ -47,17 +48,36 @@ let load_acc_lemma2 b acc0 r =
   let c0 = pfadd (pow2 128) (nat_from_bytes_le b0) in
   let c1 = pfadd (pow2 128) (nat_from_bytes_le b1) in
 
-  FStar.Math.Lemmas.modulo_lemma c1 prime;
+  Math.Lemmas.modulo_lemma c1 prime;
+  Math.Lemmas.multiple_modulo_lemma 2 size_block;
 
   let f = S.poly1305_update1 r size_block in
   let nb = (2 * size_block) / size_block in
+  Math.Lemmas.cancel_mul_div 2 size_block;
+  assert (nb == 2);
+
   let repeat_f = repeat_blocks_f size_block b f nb in
 
-  lemma_repeat_blocks_multi size_block b f acc0;
-  Loops.unfold_repeati nb repeat_f acc0 1;
-  Loops.unfold_repeati nb repeat_f acc0 0;
-  Loops.eq_repeati0 nb repeat_f acc0;
-  Lemmas.poly_update_multi_lemma_load2_simplify acc0 r c0 c1
+  calc (==) {
+    repeat_blocks_multi size_block b f acc0;
+    (==) { lemma_repeat_blocks_multi size_block b f acc0 }
+    Lib.LoopCombinators.repeati nb repeat_f acc0;
+    (==) { Loops.unfold_repeati nb repeat_f acc0 1;
+           Loops.unfold_repeati nb repeat_f acc0 0;
+           Loops.eq_repeati0 nb repeat_f acc0
+         }
+    repeat_f 1 (repeat_f 0 acc0);
+    (==) {
+      Math.Lemmas.mul_one_left_is_same size_block;
+      assert (b1 == Seq.slice b (1 * size_block) (1 * size_block + size_block)) }
+    f b1 (f b0 acc0);
+    (==) {
+      assert_norm (8 * size_block == 128);
+      Lemmas.poly_update_multi_lemma_load2_simplify acc0 r c0 c1 }
+    normalize_2 r (load_acc b acc0);
+    (==) { }
+    normalize_n r (load_acc b acc0);
+  }
 
 
 val load_acc_lemma4: b:block_v 4 -> acc0:pfelem -> r:pfelem -> Lemma
@@ -75,26 +95,42 @@ let load_acc_lemma4 b acc0 r =
   let c2 = pfadd (pow2 128) (nat_from_bytes_le b2) in
   let c3 = pfadd (pow2 128) (nat_from_bytes_le b3) in
 
-  FStar.Math.Lemmas.modulo_lemma c1 prime;
-  FStar.Math.Lemmas.modulo_lemma c2 prime;
-  FStar.Math.Lemmas.modulo_lemma c3 prime;
+  Math.Lemmas.modulo_lemma c1 prime;
+  Math.Lemmas.modulo_lemma c2 prime;
+  Math.Lemmas.modulo_lemma c3 prime;
 
   let f = S.poly1305_update1 r size_block in
   let nb = (4 * size_block) / size_block in
+  Math.Lemmas.cancel_mul_div 4 size_block;
+  assert (nb == 4);
   let repeat_f = repeat_blocks_f size_block b f nb in
 
-  lemma_repeat_blocks_multi size_block b f acc0;
-  Loops.unfold_repeati nb repeat_f acc0 3;
-  Loops.unfold_repeati nb repeat_f acc0 2;
-  Loops.unfold_repeati nb repeat_f acc0 1;
-  Loops.unfold_repeati nb repeat_f acc0 0;
-  Loops.eq_repeati0 nb repeat_f acc0;
-  Lemmas.poly_update_multi_lemma_load4_simplify acc0 r c0 c1 c2 c3
+  Math.Lemmas.multiple_modulo_lemma 4 size_block;
+  calc (==) {
+    repeat_blocks_multi size_block b f acc0;
+    (==) { lemma_repeat_blocks_multi size_block b f acc0 }
+    Lib.LoopCombinators.repeati nb repeat_f acc0;
+    (==) {
+      Loops.unfold_repeati nb repeat_f acc0 3;
+      Loops.unfold_repeati nb repeat_f acc0 2;
+      Loops.unfold_repeati nb repeat_f acc0 1;
+      Loops.unfold_repeati nb repeat_f acc0 0;
+      Loops.eq_repeati0 nb repeat_f acc0
+    }
+    repeat_f 3 (repeat_f 2 (repeat_f 1 (repeat_f 0 acc0)));
+    (==) { Math.Lemmas.mul_one_left_is_same size_block }
+    f b3 (f b2 (f b1 (f b0 acc0)));
+    (==) {
+      assert_norm (8 * size_block == 128);
+      Lemmas.poly_update_multi_lemma_load4_simplify acc0 r c0 c1 c2 c3
+    }
+    normalize_n r (load_acc b acc0);
+  }
 
-
-val load_acc_lemma: #w:lanes -> b:block_v w -> acc0:pfelem -> r:pfelem -> Lemma
-  (normalize_n r (load_acc b acc0) ==
-   repeat_blocks_multi size_block b (S.poly1305_update1 r size_block) acc0)
+val load_acc_lemma: #w:lanes{w * size_block <= max_size_t} -> b:block_v w -> acc0:pfelem -> r:pfelem -> Lemma
+  (Math.Lemmas.multiple_modulo_lemma w size_block;
+   normalize_n r (load_acc b acc0) ==
+     repeat_blocks_multi size_block b (S.poly1305_update1 r size_block) acc0)
 
 let load_acc_lemma #w b acc0 r =
   match w with
@@ -111,6 +147,7 @@ let load_acc_lemma #w b acc0 r =
 
 val poly_update_nblocks_lemma1: r:pfelem -> b:block_v 1 -> acc_v0:elem 1 -> Lemma
   (let rw = compute_rw #1 r in
+   Math.Lemmas.multiple_modulo_lemma 1 size_block;
    normalize_n r (poly1305_update_nblocks rw b acc_v0) ==
    repeat_blocks_multi size_block b (S.poly1305_update1 r size_block) (normalize_n r acc_v0))
 
@@ -132,6 +169,7 @@ val poly_update_nblocks_lemma2: r:pfelem -> b:block_v 2 -> acc_v0:elem 2 -> Lemm
 
 let poly_update_nblocks_lemma2 r b acc_v0 =
   let acc0 = normalize_n r acc_v0 in
+  let rw = compute_rw #2 r in
   let b0 = Seq.slice b 0 size_block in
   let b1 = Seq.slice b size_block (2 * size_block) in
   let c0 = pfadd (pow2 128) (nat_from_bytes_le b0) in
@@ -139,15 +177,29 @@ let poly_update_nblocks_lemma2 r b acc_v0 =
 
   let f = S.poly1305_update1 r size_block in
   let nb = (2 * size_block) / size_block in
+  Math.Lemmas.cancel_mul_div 2 size_block;
+  assert (nb == 2);
   let repeat_f = repeat_blocks_f size_block b f nb in
 
-  lemma_repeat_blocks_multi size_block b f acc0;
-  Loops.unfold_repeati nb repeat_f acc0 1;
-  Loops.unfold_repeati nb repeat_f acc0 0;
-  Loops.eq_repeati0 nb repeat_f acc0;
-  Lemmas.poly_update_multi_lemma_load2_simplify acc0 r c0 c1;
-  Lemmas.poly_update_repeat_blocks_multi_lemma2_simplify acc_v0.[0] acc_v0.[1] c0 c1 r
-
+  Math.Lemmas.multiple_modulo_lemma 2 size_block;
+  calc (==) {
+    repeat_blocks_multi size_block b f acc0;
+    (==) { lemma_repeat_blocks_multi size_block b f acc0 }
+    Lib.LoopCombinators.repeati nb repeat_f acc0;
+    (==) {
+      Loops.unfold_repeati nb repeat_f acc0 1;
+      Loops.unfold_repeati nb repeat_f acc0 0;
+      Loops.eq_repeati0 nb repeat_f acc0;
+      Math.Lemmas.mul_one_left_is_same size_block
+    }
+    f b1 (f b0 acc0);
+    (==) {
+      assert_norm (8 * size_block == 128);
+      Lemmas.poly_update_multi_lemma_load2_simplify acc0 r c0 c1;
+      Lemmas.poly_update_repeat_blocks_multi_lemma2_simplify acc_v0.[0] acc_v0.[1] c0 c1 r
+    }
+    normalize_n r (poly1305_update_nblocks rw b acc_v0);
+  }
 
 val poly_update_nblocks_lemma4: r:pfelem -> b:block_v 4 -> acc_v0:elem 4 -> Lemma
   (let rw = compute_rw #4 r in
@@ -156,6 +208,7 @@ val poly_update_nblocks_lemma4: r:pfelem -> b:block_v 4 -> acc_v0:elem 4 -> Lemm
 
 let poly_update_nblocks_lemma4 r b acc_v0 =
   let acc0 = normalize_n r acc_v0 in
+  let rw = compute_rw #4 r in
   let b0 = Seq.slice b 0 size_block in
   let b1 = Seq.slice b size_block (2 * size_block) in
   let b2 = Seq.slice b (2 * size_block) (3 * size_block) in
@@ -171,21 +224,37 @@ let poly_update_nblocks_lemma4 r b acc_v0 =
 
   let f = S.poly1305_update1 r size_block in
   let nb = (4 * size_block) / size_block in
+  Math.Lemmas.cancel_mul_div 4 size_block;
+  assert (nb == 4);
   let repeat_f = repeat_blocks_f size_block b f nb in
 
-  lemma_repeat_blocks_multi size_block b f acc0;
-  Loops.unfold_repeati nb repeat_f acc0 3;
-  Loops.unfold_repeati nb repeat_f acc0 2;
-  Loops.unfold_repeati nb repeat_f acc0 1;
-  Loops.unfold_repeati nb repeat_f acc0 0;
-  Loops.eq_repeati0 nb repeat_f acc0;
+  Math.Lemmas.multiple_modulo_lemma 4 size_block;
+  calc (==) {
+    repeat_blocks_multi size_block b f acc0;
+    (==) { lemma_repeat_blocks_multi size_block b f acc0 }
+    Lib.LoopCombinators.repeati nb repeat_f acc0;
+    (==) {
+      Loops.unfold_repeati nb repeat_f acc0 3;
+      Loops.unfold_repeati nb repeat_f acc0 2;
+      Loops.unfold_repeati nb repeat_f acc0 1;
+      Loops.unfold_repeati nb repeat_f acc0 0;
+      Loops.eq_repeati0 nb repeat_f acc0
+    }
+    repeat_f 3 (repeat_f 2 (repeat_f 1 (repeat_f 0 acc0)));
+    (==) { Math.Lemmas.mul_one_left_is_same size_block }
+    f b3 (f b2 (f b1 (f b0 acc0)));
+    (==) {
+      assert_norm (8 * size_block == 128);
+      Lemmas.poly_update_repeat_blocks_multi_lemma4_simplify
+        acc_v0.[0] acc_v0.[1] acc_v0.[2] acc_v0.[3] c0 c1 c2 c3 r r2 r4
+    }
+   normalize_n r (poly1305_update_nblocks rw b acc_v0);
+  }
 
-  Lemmas.poly_update_repeat_blocks_multi_lemma4_simplify
-    acc_v0.[0] acc_v0.[1] acc_v0.[2] acc_v0.[3] c0 c1 c2 c3 r r2 r4
 
-
-val poly_update_nblocks_lemma: #w:lanes -> r:pfelem -> b:block_v w -> acc_v0:elem w -> Lemma
+val poly_update_nblocks_lemma: #w:lanes{w * size_block <= max_size_t} -> r:pfelem -> b:block_v w -> acc_v0:elem w -> Lemma
   (let rw = compute_rw #w r in
+   Math.Lemmas.multiple_modulo_lemma w size_block;
    normalize_n r (poly1305_update_nblocks rw b acc_v0) ==
    repeat_blocks_multi size_block b (S.poly1305_update1 r size_block) (normalize_n r acc_v0))
 
@@ -196,7 +265,7 @@ let poly_update_nblocks_lemma #w r b acc_v0 =
   | 4 -> poly_update_nblocks_lemma4 r b acc_v0
 
 
-val repeat_blocks_multi_vec_equiv_pre_lemma: #w:lanes -> r:pfelem -> b:block_v w -> acc_v0:elem w -> Lemma
+val repeat_blocks_multi_vec_equiv_pre_lemma: #w:lanes{w * size_block <= max_size_t} -> r:pfelem -> b:block_v w -> acc_v0:elem w -> Lemma
   (let rw = compute_rw #w r in
    let f = S.poly1305_update1 r size_block in
    let f_v = poly1305_update_nblocks rw in
@@ -207,7 +276,7 @@ let repeat_blocks_multi_vec_equiv_pre_lemma #w r b acc_v0 =
 
 
 val poly_update_multi_lemma_v:
-    #w:lanes
+    #w:lanes{w * size_block > 0 /\ w * size_block <= max_size_t}
   -> text:bytes{length text % (w * size_block) = 0 /\ length text % size_block = 0}
   -> acc_v0:elem w
   -> r:pfelem -> Lemma
@@ -227,7 +296,7 @@ let poly_update_multi_lemma_v #w text acc_v0 r =
 
 
 val poly_update_multi_lemma:
-    #w:lanes
+    #w:lanes{w * size_block > 0 /\ w * size_block <= max_size_t}
   -> text:bytes{w * size_block <= length text /\ length text % (w * size_block) = 0 /\ length text % size_block = 0}
   -> acc0:pfelem
   -> r:pfelem -> Lemma
@@ -237,10 +306,12 @@ val poly_update_multi_lemma:
 let poly_update_multi_lemma #w text acc0 r =
   let len = length text in
   let blocksize_v = w * size_block in
+  Math.Lemmas.cancel_mul_mod w size_block;
   let text0 = Seq.slice text 0 blocksize_v in
   let text1 = Seq.slice text blocksize_v len in
-  FStar.Math.Lemmas.modulo_addition_lemma len blocksize_v (- 1);
-  assert (length text1 % (w * size_block) = 0 /\ length text1 % size_block = 0);
+  Math.Lemmas.modulo_addition_lemma len blocksize_v (- 1);
+  Math.Lemmas.euclidean_division_definition len size_block;
+  assert (length text1 % size_block = 0);
 
   let f = S.poly1305_update1 r size_block in
   let acc_v0 = load_acc #w text0 acc0 in
@@ -257,19 +328,37 @@ val poly1305_update_vec_lemma: #w:lanes -> text:bytes -> acc0:pfelem -> r:pfelem
 let poly1305_update_vec_lemma #w text acc0 r =
   let len = length text in
   let blocksize_v = w * size_block in
+  Math.Lemmas.pos_times_pos_is_pos w size_block;
   let len0 = len / blocksize_v * blocksize_v in
-  FStar.Math.Lemmas.cancel_mul_mod (len / blocksize_v) blocksize_v;
+  Math.Lemmas.cancel_mul_mod (len / blocksize_v) blocksize_v;
   assert (len0 % blocksize_v = 0);
+  Math.Lemmas.paren_mul_right (len/blocksize_v) w size_block;
+  assert (len0 == ((len / blocksize_v) * w) * size_block);
   assert (len0 % size_block = 0);
 
+  Math.Lemmas.nat_over_pos_is_nat len blocksize_v;
+  Math.Lemmas.nat_times_nat_is_nat (len/blocksize_v) blocksize_v;
+  assert (0 <= len0);
+  Math.Lemmas.euclidean_division_definition len blocksize_v;
+  assert (len0 <= len);
   let text0 = Seq.slice text 0 len0 in
   let f = S.poly1305_update1 r size_block in
   let l = S.poly1305_update_last r in
 
-  if len0 > 0 then begin
+  assert_norm (1 * size_block > 0 /\ 1 * size_block <= max_size_t);
+  assert_norm (2 * size_block > 0 /\ 2 * size_block <= max_size_t);
+  assert_norm (4 * size_block > 0 /\ 4 * size_block <= max_size_t);
+  assert (w * size_block > 0 /\ w * size_block <= max_size_t);
+  if len / blocksize_v > 0 then begin
+    Math.Lemmas.lemma_mult_le_right blocksize_v 1 (len / blocksize_v);
+    assert (blocksize_v <= len0);
     poly_update_multi_lemma #w text0 acc0 r;
-    SeqLemmas.repeat_blocks_split size_block len0 text f l acc0 end
-
+    SeqLemmas.repeat_blocks_split size_block len0 text f l acc0
+    end
+  else begin
+    Math.Lemmas.mul_zero_left_is_zero blocksize_v;
+    assert (len0 == 0)
+  end
 
 val poly1305_vec_lemma: #w:lanes -> msg:bytes -> k:S.key ->
   Lemma (poly1305_mac #w msg k == S.poly1305_mac msg k)
